examples/wysteria/prog.ml
@@ -1,3 +1,5 @@
 open AST
 
+open FFI
+  
 let program = E_const (C_unit ())
